Write some code that isn't used yet
We can now automatically infer the bin-op and brackets, but that makes
[simpl] stack-overflow.

We also factor the [string] out of the recursive call.  This is
currently untested, because I only tried testing it with the above
turned on.

src/Parsers/BooleanRecognizerOptimized.v
@@ -7,6 +7,7 @@ Require Import Fiat.Parsers.BaseTypes.
 Require Import Fiat.Parsers.StringLike.Properties.
 Require Import Fiat.Common Fiat.Common.Wf.
 Require Import Fiat.Parsers.BooleanRecognizer.
+Require Import Fiat.Parsers.BooleanRecognizerCorrect.
 Require Import Fiat.Common.Match.
 Require Import Fiat.Common.List.ListFacts.
 Require Import Fiat.Common.Equality.
@@ -46,12 +47,39 @@ Local Ltac simpl_setoid_rewrite lem :=
     clear H.
 
 Section recursive_descent_parser.
-  Context {Char} {HSL : StringLike Char}
+  Context {Char} {HSL : StringLike Char} {HSLP : StringLikeProperties Char}
           {ls : list (String.string * productions Char)}.
   Context {data : @boolean_parser_dataT Char _}.
+
+  Class str_carrier (constT varT : Type)
+    := { to_string : constT * varT -> String;
+         of_string : String -> constT * varT;
+         to_of : forall x, to_string (of_string x) = x;
+         of_to : forall x, of_string (to_string x) = x;
+         drop_const : forall x n, fst (of_string (drop n x)) = fst (of_string x);
+         take_const : forall x n, fst (of_string (take n x)) = fst (of_string x)}.
+
+  Definition str_carrier' (constT varT : Type)
+    := { to_string : constT * varT -> StringLike.String
+       & { of_string : StringLike.String -> constT * varT
+         | (forall x, to_string (of_string x) = x)
+           /\ (forall x, of_string (to_string x) = x)
+           /\ (forall x n, fst (of_string (drop n x)) = fst (of_string x))
+           /\ (forall x n, fst (of_string (take n x)) = fst (of_string x)) } }.
+
+  Definition str_carrier_default {constT varT} (strC : str_carrier' constT varT)
+  : str_carrier constT varT.
+  Proof.
+    refine {| to_string := projT1 strC;
+              of_string := proj1_sig (projT2 strC) |};
+    apply (proj2_sig (projT2 strC)).
+  Defined.
+
+  Context constT varT {strC : str_carrier constT varT}.
+
   Local Notation G := (list_to_grammar (nil::nil) ls) (only parsing).
 
-  Definition parse_nonterminal_opt
+  Definition parse_nonterminal_opt'
              (str : String)
              (nt : String.string)
   : { b : bool | b = parse_nonterminal (G := G) str nt }.
@@ -123,4 +151,166 @@ Section recursive_descent_parser.
       subst e; instantiate.
     reflexivity.
   Defined.
+
+  Lemma take_drop_helper n ms x
+  : take n (fold_right drop (to_string x) ms)
+    = to_string (fst x,
+                 snd (of_string (take n (fold_right drop (to_string x) ms)))).
+  Proof.
+    rewrite <- (rev_involutive ms).
+    rewrite fold_left_rev_right.
+    generalize (rev ms); clear ms; intro ms.
+    revert n x; induction ms; intros n [x y]; simpl.
+    { match goal with
+        | [ |- ?x = ?y ]
+          => etransitivity;
+            [ symmetry; exact (to_of x)
+            | etransitivity; [ | exact (to_of y) ] ]
+      end.
+      apply f_equal.
+      apply injective_projections.
+      { rewrite take_const, !of_to; reflexivity. }
+      { rewrite !of_to; simpl; reflexivity. } }
+    { pose proof (IHms n (of_string (drop a (to_string (x, y))))) as IHms'.
+      rewrite to_of in IHms'.
+      rewrite IHms'; clear IHms'.
+      rewrite drop_const, !of_to; simpl.
+      reflexivity. }
+  Qed.
+
+  Definition parse_nonterminal_opt''
+             (str : String)
+             (nt : String.string)
+  : { b : bool | b = parse_nonterminal (G := G) str nt }.
+  Proof.
+    eexists.
+    transitivity (proj1_sig (parse_nonterminal_opt' str nt)); [ | exact (proj2_sig (parse_nonterminal_opt' str nt)) ].
+    cbv beta iota zeta delta [parse_nonterminal_opt' proj1_sig].
+    lazymatch goal with
+      | [ |- ?e = Fix
+                    ?wf
+                    (fun (a : ?T0) => ?T1 -> String -> ?T2)
+                    (fun (a' : ?T0)
+                         (x : forall a'' : ?T0,
+                                ?R a'' a'
+                                -> ?T1 -> String -> @?T2' a'')
+                         (y : ?T1)
+                         (z : String)
+                     => @?f a' x y z)
+                    ?v1 ?v2 ?str ?v4 ?v5 ?v6 ]
+        => let f' := constr:(fun const_str
+                                 (a' : T0)
+                                 (x : forall a'' : T0, R a'' a' -> T1 -> varT -> T2' a'')
+                                 (y : T1)
+                                 (z : varT)
+                             => f a' (fun a'' rwf t1 str'
+                                      => x a'' rwf t1 (snd (of_string str')))
+                                  y (to_string (const_str, z))) in
+           let vstr' := constr:(snd (of_string str)) in
+           let f'h := fresh "f0" in
+           let fh := fresh "f1" in
+           set (f'h := f');
+             set (fh := f);
+             let GT := constr:(Fix
+                                 wf
+                                 (fun (a : T0) => T1 -> varT -> T2)
+                                 (f'h (fst (of_string str)))
+                                 v1 v2 vstr' v4 v5 v6
+                               = Fix
+                                   wf
+                                   (fun (a : T0) => T1 -> String -> T2)
+                                   fh
+                                   v1 v2 str v4 v5 v6) in
+             refine (_ : GT); change GT;
+             let H := fresh in
+             assert (H : forall a b vstr' d e f0,
+                           Fix wf (fun (a : T0) => T1 -> varT -> T2) (f'h (fst (of_string str))) a b vstr' d e f0
+                           = Fix wf (fun (a : T0) => T1 -> String -> T2) fh a b (to_string (fst (of_string str), vstr')) d e f0);
+               [ let a := fresh in intro a; induction (wf a) as [?? IH]
+               | specialize (fun a b => H a b (snd (of_string str)));
+                 rewrite <- surjective_pairing in H;
+                 rewrite to_of in H;
+                 rewrite <- H;
+                 reflexivity ]
+    end.
+    intros.
+    rewrite !Fix5_eq;
+      [ unfold f0 at 1, f1 at 1
+      | unfold f0, f1
+      | unfold f0, f1 ];
+      repeat match goal with
+               | _ => progress intros
+               | [ |- ?x = ?x ] => reflexivity
+               | [ |- fold_right _ _ _ = fold_right _ _ _ ]
+                 => apply fold_right_f_eq_mor; [ intros ?? | | ]
+               | [ |- (match ?x with _ => _ end) = (match ?x with _ => _ end) ]
+                 => destruct x eqn:?
+               | [ |- (match ?x with _ => _ end) _ _ _ _ = (match ?x with _ => _ end) _ _ _ _ ]
+                 => destruct x eqn:?
+               | [ H : fst (of_string _) = ?x |- context[?x] ] => rewrite <- H
+               | [ |- fold_left _ _ _ = fold_left _ _ _ ]
+                 => rewrite <- !fold_left_rev_right
+               | [ |- rev _ = rev _ ]
+                 => apply f_equal
+               | [ |- map _ ?ls = map _ ?ls ]
+                 => apply map_ext; intro
+               | [ |- EqNat.beq_nat ?x ?y = EqNat.beq_nat ?x' ?y ]
+                 => apply f_equal2
+               | [ |- context[(fst ?x, snd ?x)] ]
+                 => rewrite <- surjective_pairing
+               | [ |- context[to_string (of_string _)] ]
+                 => rewrite to_of
+               | [ |- context[of_string (to_string _)] ]
+                 => rewrite of_to
+               | [ H : context[(fst ?x, snd ?x)] |- _ ]
+                 => rewrite <- surjective_pairing in H
+               | [ H : context[to_string (of_string _)] |- _ ]
+                 => rewrite to_of in H
+               | [ |- parse_production' _ _ _ _ = parse_production' _ _ _ _ ]
+                 => apply parse_production_drop_ext with (ms := nil); intros
+               | [ |- _ = Fix _ _ _ _ _ (take ?n (fold_right drop (?f ?x) ?ms)) _ _ _ ]
+                 => rewrite (take_drop_helper n ms x : take n (fold_right drop (f x) ms) = _)
+               | _ => progress simpl in *
+               | _ => congruence
+               | [ |- Fix _ _ _ ?a ?b ?c ?d ?e ?f = _ ]
+                 => specialize (fun H' => IH a H' b c d e f);
+                   try match goal with
+                         | [ H : _ |- _ ] => specialize (IH (or_introl H))
+                       end;
+                   try apply IH
+               | [ |- prod_relation _ _ _ _ ] => hnf
+               | [ H : (_ && _)%bool = true |- _ ] => apply Bool.andb_true_iff in H
+               | [ H : _ = in_left |- _ ] => clear H
+               | [ H : _ /\ _ |- _ ] => destruct H
+               | [ H : context[negb (EqNat.beq_nat ?x ?y)] |- _ ] => destruct (EqNat.beq_nat x y) eqn:?
+               | [ H : EqNat.beq_nat _ _ = false |- _ ] => apply EqNat.beq_nat_false in H
+               | [ |- _ \/ _ ] => right; split; [ reflexivity | omega ]
+             end.
+  Defined.
+
+  Definition parse_nonterminal_opt
+             (str : String)
+             (nt : String.string)
+  : { b : bool | b = parse_nonterminal (G := G) str nt }.
+  Proof.
+    let impl := (eval cbv beta iota zeta delta [parse_nonterminal_opt'' proj1_sig] in (proj1_sig (parse_nonterminal_opt'' str nt))) in
+    (exists impl).
+    abstract (exact (proj2_sig (parse_nonterminal_opt'' str nt))).
+  Defined.
 End recursive_descent_parser.
+
+(** This tactic solves the simple case where the type of string is
+    judgmentally [const_data * variable_data], and [take] and [drop]
+    judgmentally preserve the constant data. *)
+
+Ltac solve_default_str_carrier :=
+  match goal with |- str_carrier _ _ => idtac end;
+  eapply str_carrier_default; hnf; simpl;
+  match goal with |- { to_string : _ * _ -> string * _ & _ } => idtac end;
+  let T := match goal with |- { to_string : _ * _ -> string * ?T & _ } => constr:T end in
+  exists (fun x : string * T => x);
+    exists (fun x : string * T => x);
+    simpl;
+    solve [ repeat split ].
+
+Hint Extern 1 (str_carrier _ _) => solve_default_str_carrier : typeclass_instances.
